# 有限微积分与数列求和

## 差分

定义:
$$
\begin{align*}
\Delta f(x) &= f(x + 1) - f(x)\\
f(x) &= \Delta F(x)\\
\operatorname{E}f(x) &= f(x + 1)
\end{align*}
$$
则:
$$
\begin{align*}
\Delta \big(f \pm g\big) &= f(x + 1) \pm g(x + 1) - \big(f(x)\pm g(x)\big)\\
&=\big(f(x + 1) - f(x)\big) \pm \big(g(x + 1) - g(x)\big)\\
&=\Delta f \pm \Delta g\\
\Delta\big(Cf\big)&=Cf(x + 1) - Cf(x)\\
&=C\big(f(x + 1) - f(x)\big)\\
&=C\Delta f\\
\Delta (fg)&=f(x + 1)g(x + 1) - f(x)g(x)\\
&=f(x + 1)g (x + 1) - f(x)g(x + 1) + f(x)g(x + 1)-f(x)g(x)\\
&=\operatorname{E}g\Delta f + f\Delta g
\end{align*}
$$

## 定和式

定义：

$$\sum_a^bf(x)\delta x = \sum_{k = a}^{b - 1}f(k)$$

则：

$$
\begin{align*}
\sum_a^b\Delta f(x)\delta x &=\Delta f(a) + \Delta f(a + 1) + \cdots + \Delta f(b - 1)\\
&=f(a + 1) - f(a) = f(a + 2) - f(a + 1) + \cdots + f(b) - f(b - 1)\\
&=f(b) - f(a)\\
\sum_a^af(x)\delta x&=0\\
\sum_a^bf(x)\delta x &= F(b) - F(a)\\
&= -\big(F(a) - f(b)\big)\\
&=-\sum_b^af(x)\delta x\\
\sum_a^bf(x)\delta x + \sum_b^c f(x)\delta x&= \big(F(b) - F(a)\big) + \big(F(c) - F(b)\big)\\
&=F(c) - F(a)\\
&=\sum_a^cf(x)\delta x\\
\sum_a^bf(x)\delta x \pm \sum_a^bg(x)\delta x &=\big(F(b) - F(a)\big) \pm \big(G(b) - G(a)\big)\\
&=\big(F(b)\pm G(b)\big) - \big(F(a)\pm G(a)\big)\\
&=\sum_a^b\big(f(x) \pm g(x)\big) \delta x\\
\sum_a^bCf(x)\delta x&=CF(b) - CF(a)\\
&=C\big(F(b) - F(a)\big)\\
&=C\sum_a^bf(x)\delta x\\
\end{align*}
$$

## 例题

### 例1

计算$\sum\limits_{k = 0}^{n-1}a^k(a为常数且a\ne 0)$
$$
\begin{align*}
\Delta \left(a^x\right)&=a^{x+1}-a^x\\
&=(a-1)a^x\\
\therefore a^x&=\frac{\Delta\left(a^x\right)}{a-1}\\
&=\Delta\left(\frac{a^x}{a-1}\right)\\
\therefore \sum_{k=0}^{n-1}a^k&=\sum_0^{n}a^k\delta x\\
&=\sum_0^{n}\Delta \left(\frac{a^x}{a-1}\right)\delta x\\
&=\frac{a^{n}}{a-1} - \frac{a^0}{a-1}\\
&=\frac{a^{n}-1}{a-1}
\end{align*}
$$